<?xml version="1.0" encoding="UTF-8"?>
<!--
Copyright (c) 2012, University of Texas at El Paso
All rights reserved.
Redistribution and use in source and binary forms, with or without 
modification, are permitted provided that the following conditions are met:
- Redistributions of source code must retain the above copyright notice, this 
  list of conditions and the following disclaimer.
- Redistributions in binary form must reproduce the above copyright notice, 
  this list of conditions and the following disclaimer in the documentation 
  and/or other materials provided with the distribution.
  
  THIS SOFTWARE IS PROVIDED BY THE COPYRIGHT HOLDERS AND CONTRIBUTORS "AS IS" 
  AND ANY EXPRESS OR IMPLIED WARRANTIES, INCLUDING, BUT NOT LIMITED TO, THE 
  IMPLIED WARRANTIES OF MERCHANTABILITY AND FITNESS FOR A PARTICULAR PURPOSE 
  ARE DISCLAIMED. IN NO EVENT SHALL THE COPYRIGHT HOLDER OR CONTRIBUTORS BE 
  LIABLE FOR ANY DIRECT, INDIRECT, INCIDENTAL, SPECIAL, EXEMPLARY, OR 
  CONSEQUENTIAL DAMAGES (INCLUDING, BUT NOT LIMITED TO, PROCUREMENT OF 
  SUBSTITUTE GOODS OR SERVICES; LOSS OF USE, DATA, OR PROFITS; OR BUSINESS 
  INTERRUPTION) HOWEVER CAUSED AND ON ANY THEORY OF LIABILITY, WHETHER IN 
  CONTRACT, STRICT LIABILITY, OR TORT (INCLUDING NEGLIGENCE OR OTHERWISE) 
  ARISING IN ANY WAY OUT OF THE USE OF THIS SOFTWARE, EVEN IF ADVISED OF THE 
  POSSIBILITY OF SUCH DAMAGE.
 */
-->
<!DOCTYPE rdf:RDF [
  <!ENTITY owl "http://www.w3.org/2002/07/owl#">
  <!ENTITY pml-provenance "http://inference-web.org/2.0/pml-provenance.owl">
  <!ENTITY rdf "http://www.w3.org/1999/02/22-rdf-syntax-ns#">
  <!ENTITY rdfs "http://www.w3.org/2000/01/rdf-schema#">
  <!ENTITY wdo "http://trust.utep.edu/2.0/wdo.owl">
  <!ENTITY xsd "http://www.w3.org/2001/XMLSchema#">
]>
<rdf:RDF xml:base="&wdo;"
         xmlns:owl="&owl;"
         xmlns:rdf="&rdf;"
         xmlns:rdfs="&rdfs;">

<!-- Ontology Information -->
  <owl:Ontology rdf:about="">
    <rdfs:comment xml:lang="en">The Workflow-Driven Ontology</rdfs:comment>
    <rdfs:label xml:lang="en">Workflow-Driven Ontology</rdfs:label>
    <owl:imports>
      <owl:Ontology rdf:about="&pml-provenance;"/>
    </owl:imports>
    <owl:versionInfo xml:lang="en">Version 2.0 of the Workflow Driven Ontology. Authors: Leonardo Salayandia, Ann Q. Gates, and Paulo Pinheiro da Silva</owl:versionInfo>
  </owl:Ontology>

<!-- Change log:
     Version 2.0.0: Aligned to the pmlp ontology. wdo:Data was replaced by pmlp:Information, and wdo:Method was replaced by pmlp:MethodRule.
                    The intention is to facilitate pml encoding through SAWs, as well as to reuse the same vocabulary of the WDO to query provenace.
                
     Version 2.0.1:	Added data property hasSubclassOrder to facilitate the presentation of concept hierarchy trees.
     Version 2.1.0: Added the class WorkflowDrivenOntology and made the class SemanticAbstractWorkflow a subclass of owl:Ontology. The intention is to subclass the owl:Ontology class as one of these classes to identify the type of OWL document.
-->

<!-- Classes -->
  <owl:Class rdf:about="#WorkflowDrivenOntology">
    <rdfs:comment xml:lang="en">Workflow Driven Ontologies contain process-related concepts.</rdfs:comment>
    <rdfs:label xml:lang="en">WDO</rdfs:label>
    <rdfs:subClassOf rdf:resource="&owl;Ontology"/>
  </owl:Class>
  
  <owl:Class rdf:about="&pml-provenance;#Information">
    <rdfs:comment xml:lang="en">Data and dataset concepts of the domain being modeled. Aligned to the pmlp:Information concept.</rdfs:comment>
    <rdfs:label xml:lang="en">Data</rdfs:label>
    <rdfs:subClassOf>
      <owl:Restriction>
        <owl:allValuesFrom rdf:resource="&pml-provenance;#MethodRule"/>
        <owl:onProperty rdf:resource="#isInputTo"/>
      </owl:Restriction>
    </rdfs:subClassOf>
    <rdfs:subClassOf>
      <owl:Restriction>
        <owl:allValuesFrom rdf:resource="&pml-provenance;#MethodRule"/>
        <owl:onProperty rdf:resource="#isOutputOf"/>
      </owl:Restriction>
    </rdfs:subClassOf>
    <rdfs:subClassOf>
      <owl:Restriction>
        <owl:allValuesFrom rdf:resource="&pml-provenance;#Information"/>
        <owl:onProperty rdf:resource="#isComposedOf"/>
      </owl:Restriction>
    </rdfs:subClassOf>
    <rdfs:subClassOf>
      <owl:Restriction>
        <owl:allValuesFrom rdf:resource="&pml-provenance;#Information"/>
        <owl:onProperty rdf:resource="#isPartOf"/>
      </owl:Restriction>
    </rdfs:subClassOf>
    <rdfs:subClassOf>
      <owl:Restriction>
        <owl:allValuesFrom rdf:resource="&pml-provenance;#Source"/>
        <owl:onProperty rdf:resource="#hasSource"/>
      </owl:Restriction>
    </rdfs:subClassOf>
    <rdfs:subClassOf>
      <owl:Restriction>
        <owl:maxCardinality rdf:datatype="&xsd;nonNegativeInteger">1</owl:maxCardinality>
        <owl:onProperty rdf:resource="#hasSource"/>
      </owl:Restriction>
    </rdfs:subClassOf>
    <rdfs:subClassOf>
      <owl:Restriction>
        <owl:allValuesFrom rdf:resource="&pml-provenance;#Source"/>
        <owl:onProperty rdf:resource="#hasSink"/>
      </owl:Restriction>
    </rdfs:subClassOf>
    <rdfs:subClassOf>
      <owl:Restriction>
        <owl:maxCardinality rdf:datatype="&xsd;nonNegativeInteger">1</owl:maxCardinality>
        <owl:onProperty rdf:resource="#hasSink"/>
      </owl:Restriction>
    </rdfs:subClassOf>
    <rdfs:subClassOf>
      <owl:Restriction>
        <owl:allValuesFrom rdf:resource="#RectangularCoordinate"/>
        <owl:onProperty rdf:resource="#hasLabelCoordinate"/>
      </owl:Restriction>
    </rdfs:subClassOf>
    <rdfs:subClassOf>
      <owl:Restriction>
        <owl:maxCardinality rdf:datatype="&xsd;nonNegativeInteger">1</owl:maxCardinality>
        <owl:onProperty rdf:resource="#hasLabelCoordinate"/>
      </owl:Restriction>
    </rdfs:subClassOf>
  </owl:Class>

  <owl:Class rdf:about="&pml-provenance;#MethodRule">
    <rdfs:comment xml:lang="en">Methods, algorithms and other functionality concepts of the domain being modeled. Aligned to the pmlp:MethodRule concept.</rdfs:comment>
    <rdfs:label xml:lang="en">Method</rdfs:label>
    <rdfs:subClassOf rdf:resource="#WorkflowNode"/>
    <rdfs:subClassOf>
      <owl:Restriction>
        <owl:allValuesFrom rdf:resource="&pml-provenance;#Information"/>
        <owl:onProperty rdf:resource="#hasInput"/>
      </owl:Restriction>
    </rdfs:subClassOf>
    <rdfs:subClassOf>
      <owl:Restriction>
        <owl:allValuesFrom rdf:resource="&pml-provenance;#Information"/>
        <owl:onProperty rdf:resource="#hasOutput"/>
      </owl:Restriction>
    </rdfs:subClassOf>
    <rdfs:subClassOf>
      <owl:Restriction>
        <owl:allValuesFrom rdf:resource="#SemanticAbstractWorkflow"/>
        <owl:onProperty rdf:resource="#isDetailedBy"/>
      </owl:Restriction>
    </rdfs:subClassOf>
    <rdfs:subClassOf>
      <owl:Restriction>
        <owl:maxCardinality rdf:datatype="&xsd;nonNegativeInteger">1</owl:maxCardinality>
        <owl:onProperty rdf:resource="#isDetailedBy"/>
      </owl:Restriction>
    </rdfs:subClassOf>
    <rdfs:subClassOf>
      <owl:Restriction>
        <owl:allValuesFrom rdf:resource="&pml-provenance;#InferenceEngine"/>
        <owl:onProperty rdf:resource="#hasInferenceEngine"/>
      </owl:Restriction>
    </rdfs:subClassOf>
    <rdfs:subClassOf>
      <owl:Restriction>
        <owl:maxCardinality rdf:datatype="&xsd;nonNegativeInteger">1</owl:maxCardinality>
        <owl:onProperty rdf:resource="#hasInferenceEngine"/>
      </owl:Restriction>
    </rdfs:subClassOf>
  </owl:Class>

  <owl:Class rdf:about="#SemanticAbstractWorkflow">
    <rdfs:comment xml:lang="en">Used to reference Semantic Abstract Workflows as first-class citizens. Workflows are considered abstract because the control flow is not formally specified.</rdfs:comment>
    <rdfs:label xml:lang="en">Workflow</rdfs:label>
    <rdfs:subClassOf rdf:resource="&pml-provenance;#MethodRule"/>
    <rdfs:subClassOf rdf:resource="&owl;Ontology"/>
    <rdfs:subClassOf>
      <owl:Restriction>
        <owl:allValuesFrom rdf:resource="&pml-provenance;#MethodRule"/>
        <owl:onProperty rdf:resource="#isAbstractedBy"/>
      </owl:Restriction>
    </rdfs:subClassOf>
    <rdfs:subClassOf>
      <owl:Restriction>
        <owl:maxCardinality rdf:datatype="&xsd;nonNegativeInteger">1</owl:maxCardinality>
        <owl:onProperty rdf:resource="#isAbstractedBy"/>
      </owl:Restriction>
    </rdfs:subClassOf>
    <rdfs:subClassOf>
      <owl:Restriction>
        <owl:allValuesFrom rdf:resource="&pml-provenance;#Website"/>
        <owl:onProperty rdf:resource="#hasReport"/>
      </owl:Restriction>
    </rdfs:subClassOf>
    <rdfs:subClassOf>
      <owl:Restriction>
        <owl:allValuesFrom rdf:resource="&pml-provenance;#Document"/>
        <owl:onProperty rdf:resource="#hasSupportingDocumentation"/>
      </owl:Restriction>
    </rdfs:subClassOf>
  </owl:Class>

  <owl:Class rdf:about="#RectangularCoordinate">
    <rdfs:comment xml:lang="en">Used to specify the location of an artifact in a workflow graph.</rdfs:comment>
    <rdfs:label xml:lang="en">RectCoord</rdfs:label>
    <rdfs:subClassOf>
      <owl:Restriction>
        <owl:allValuesFrom rdf:resource="&xsd;decimal"/>
        <owl:onProperty rdf:resource="#hasXCoordinateValue"/>
      </owl:Restriction>
    </rdfs:subClassOf>
    <rdfs:subClassOf>
      <owl:Restriction>
        <owl:maxCardinality rdf:datatype="&xsd;nonNegativeInteger">1</owl:maxCardinality>
        <owl:onProperty rdf:resource="#hasXCoordinateValue"/>
      </owl:Restriction>
    </rdfs:subClassOf>
    <rdfs:subClassOf>
      <owl:Restriction>
        <owl:allValuesFrom rdf:resource="&xsd;decimal"/>
        <owl:onProperty rdf:resource="#hasYCoordinateValue"/>
      </owl:Restriction>
    </rdfs:subClassOf>
    <rdfs:subClassOf>
      <owl:Restriction>
        <owl:maxCardinality rdf:datatype="&xsd;nonNegativeInteger">1</owl:maxCardinality>
        <owl:onProperty rdf:resource="#hasYCoordinateValue"/>
      </owl:Restriction>
    </rdfs:subClassOf>
    <rdfs:subClassOf>
      <owl:Restriction>
        <owl:allValuesFrom rdf:resource="&xsd;decimal"/>
        <owl:onProperty rdf:resource="#hasZCoordinateValue"/>
      </owl:Restriction>
    </rdfs:subClassOf>
    <rdfs:subClassOf>
      <owl:Restriction>
        <owl:maxCardinality rdf:datatype="&xsd;nonNegativeInteger">1</owl:maxCardinality>
        <owl:onProperty rdf:resource="#hasZCoordinateValue"/>
      </owl:Restriction>
    </rdfs:subClassOf>
  </owl:Class>
  
  <owl:Class rdf:about="#WorkflowNode">
    <rdfs:comment xml:lang="en">Used to classify the concepts that are represented by a node in a workflow graph, and hence have a location given by a coordinate.</rdfs:comment>
    <rdfs:label xml:lang="en">Node</rdfs:label>
    <rdfs:subClassOf>
      <owl:Restriction>
        <owl:allValuesFrom rdf:resource="#RectangularCoordinate"/>
        <owl:onProperty rdf:resource="#hasCoordinate"/>
      </owl:Restriction>
    </rdfs:subClassOf>
    <rdfs:subClassOf>
      <owl:Restriction>
        <owl:maxCardinality rdf:datatype="&xsd;nonNegativeInteger">1</owl:maxCardinality>
        <owl:onProperty rdf:resource="#hasCoordinate"/>
      </owl:Restriction>
    </rdfs:subClassOf>
  </owl:Class>
  
  <owl:Class rdf:about="&pml-provenance;#Source">
    <rdfs:subClassOf rdf:resource="#WorkflowNode"/>
  </owl:Class>

<!-- Datatype Properties -->
  <owl:DatatypeProperty rdf:about="#hasXCoordinateValue">
    <rdfs:domain rdf:resource="#RectangularCoordinate"/>
    <rdfs:range rdf:resource="&xsd;decimal"/>
  </owl:DatatypeProperty>

  <owl:DatatypeProperty rdf:about="#hasYCoordinateValue">
    <rdfs:domain rdf:resource="#RectangularCoordinate"/>
    <rdfs:range rdf:resource="&xsd;decimal"/>
  </owl:DatatypeProperty>

  <owl:DatatypeProperty rdf:about="#hasZCoordinateValue">
    <rdfs:domain rdf:resource="#RectangularCoordinate"/>
    <rdfs:range rdf:resource="&xsd;decimal"/>
  </owl:DatatypeProperty>
  
  <owl:DatatypeProperty rdf:about="#hasSubclassOrder">
    <rdfs:domain rdf:resource="#RectangularCoordinate"/>
    <rdfs:range rdf:resource="&xsd;string"/>
  </owl:DatatypeProperty>

<!-- Object Properties -->
  <owl:ObjectProperty rdf:about="#hasCoordinate">
    <rdfs:comment xml:lang="en">Used to specify layout position information of workflow nodes.</rdfs:comment>
    <rdfs:label xml:lang="en">has coordinate</rdfs:label>
    <rdfs:domain rdf:resource="#WorkflowNode"/>
    <rdfs:range rdf:resource="#RectangularCoordinate"/>
  </owl:ObjectProperty>
  
  <owl:ObjectProperty rdf:about="#hasLabelCoordinate">
    <rdfs:comment xml:lang="en">Used to specify layout position information of data labels.</rdfs:comment>
    <rdfs:label xml:lang="en">has coordinate</rdfs:label>
    <rdfs:domain rdf:resource="&pml-provenance;#Information"/>
    <rdfs:range rdf:resource="#RectangularCoordinate"/>
  </owl:ObjectProperty>

  <owl:ObjectProperty rdf:about="#hasInput">
    <rdfs:comment xml:lang="en">Used to specify the pmlp:Information concepts that a pmlp:MethodRule uses as inputs. Inverse of the wdo:isInputTo property.</rdfs:comment>
    <rdfs:label xml:lang="en">has input</rdfs:label>
    <rdfs:domain rdf:resource="&pml-provenance;#MethodRule"/>
    <rdfs:range rdf:resource="&pml-provenance;#Information"/>
    <owl:inverseOf rdf:resource="#isInputTo"/>
  </owl:ObjectProperty>

  <owl:ObjectProperty rdf:about="#isInputTo">
    <rdfs:comment xml:lang="en">Used to specify the pmlp:MethodRule concepts where a pmlp:Information concept can be used as input.</rdfs:comment>
    <rdfs:label xml:lang="en">is input to</rdfs:label>
    <rdfs:domain rdf:resource="&pml-provenance;#Information"/>
    <rdfs:range rdf:resource="&pml-provenance;#MethodRule"/>
    <owl:inverseOf rdf:resource="#hasInput"/>
  </owl:ObjectProperty>

  <owl:ObjectProperty rdf:about="#hasOutput">
    <rdfs:comment xml:lang="en">Used to specify the outputs of a pmlp:MethodRule concept.</rdfs:comment>
    <rdfs:label xml:lang="en">has output</rdfs:label>
    <rdfs:domain rdf:resource="&pml-provenance;#MethodRule"/>
    <rdfs:range rdf:resource="&pml-provenance;#Information"/>
    <owl:inverseOf rdf:resource="#isOutputOf"/>
  </owl:ObjectProperty>

  <owl:ObjectProperty rdf:about="#isOutputOf">
    <rdfs:comment xml:lang="en">Used to specify the pmlp:MethodRule concepts that generate a given pmlp:Information concept. Inverse of the wdo:hasOutput property.</rdfs:comment>
    <rdfs:label xml:lang="en">is output of</rdfs:label>
    <rdfs:domain rdf:resource="&pml-provenance;#Information"/>
    <rdfs:range rdf:resource="&pml-provenance;#MethodRule"/>
    <owl:inverseOf rdf:resource="#hasOutput"/>
  </owl:ObjectProperty>

  <owl:ObjectProperty rdf:about="#hasDefaultInstance">
    <rdfs:comment xml:lang="en">Used to relate default instances to classes used to model process.</rdfs:comment>
    <rdfs:label xml:lang="en">has default instance</rdfs:label>
    <rdfs:domain rdf:resource="&owl;OntClass"/>
    <rdfs:range rdf:resource="&owl;NamedIndividual"/>
    <owl:inverseOf rdf:resource="#hasOutput"/>
  </owl:ObjectProperty>

  <owl:ObjectProperty rdf:about="#hasSource">
    <rdfs:comment xml:lang="en">Used to set the pmlp:Source where pmlp:Information can come from. It is similar to the pmlp:hasSource property, except that the pmlp relation captures where it actually came from.</rdfs:comment>
    <rdfs:label xml:lang="en">has source</rdfs:label>
    <rdfs:domain rdf:resource="&pml-provenance;#Information"/>
    <rdfs:range rdf:resource="&pml-provenance;#Source"/>
  </owl:ObjectProperty>

  <owl:ObjectProperty rdf:about="#hasSink">
    <rdfs:comment xml:lang="en">Used to set the pmlp:Source of pmlp:Information can go to.</rdfs:comment>
    <rdfs:label xml:lang="en">has sink</rdfs:label>
    <rdfs:domain rdf:resource="&pml-provenance;#Information"/>
    <rdfs:range rdf:resource="&pml-provenance;#Source"/>
  </owl:ObjectProperty>

  <owl:ObjectProperty rdf:about="#isAbstractedBy">
    <rdfs:comment xml:lang="en">Used to link an wdo:SemanticAbstractWorkflow instance to a pmlp:MethodRule instance; mechanism to support subworkflows.</rdfs:comment>
    <rdfs:label xml:lang="en">is abstracted by</rdfs:label>
    <rdfs:domain rdf:resource="#SemanticAbstractWorkflow"/>
    <rdfs:range rdf:resource="&pml-provenance;#MethodRule"/>
    <owl:inverseOf rdf:resource="#isDetailedBy"/>
  </owl:ObjectProperty>

  <owl:ObjectProperty rdf:about="#isDetailedBy">
    <rdfs:comment xml:lang="en">Used to link a pmlp:MethodRule instance to a wdo:SemanticAbstractWorkflow instance; mechanism used to support subworkflows. Inverse of wdo:isAbstractedBy.</rdfs:comment>
    <rdfs:label xml:lang="en">is detailed by</rdfs:label>
    <rdfs:domain rdf:resource="&pml-provenance;#MethodRule"/>
    <rdfs:range rdf:resource="#SemanticAbstractWorkflow"/>
    <owl:inverseOf rdf:resource="#isAbstractedBy"/>
  </owl:ObjectProperty>

  <owl:ObjectProperty rdf:about="#isComposedOf">
    <rdfs:comment xml:lang="en">Used to specify abstractions between pmlp:Information concepts, e.g., Coordinate is composed of Latitude and Longitude.</rdfs:comment>
    <rdfs:label xml:lang="en">is composed of</rdfs:label>
    <rdfs:domain rdf:resource="&pml-provenance;#Information"/>
    <rdfs:range rdf:resource="&pml-provenance;#Information"/>
    <owl:inverseOf rdf:resource="#isPartOf"/>
  </owl:ObjectProperty>

  <owl:ObjectProperty rdf:about="#isPartOf">
    <rdfs:comment xml:lang="en">Used to specify abstractions between pmlp:Information concepts, e.g., Latitude is part of Coordinate, and Longitude is part of Coordinate. Inverse of wdo:isComposedOf.</rdfs:comment>
    <rdfs:label xml:lang="en">is part of</rdfs:label>
    <rdfs:domain rdf:resource="&pml-provenance;#Information"/>
    <rdfs:range rdf:resource="&pml-provenance;#Information"/>
    <owl:inverseOf rdf:resource="#isComposedOf"/>
  </owl:ObjectProperty>
  
  <owl:ObjectProperty rdf:about="#hasInferenceEngine">
    <rdfs:comment xml:lang="en">Used to set the pmlp:InferenceEngine of a pmlp:MethodRule instance.</rdfs:comment>
    <rdfs:label xml:lang="en">has inference engine</rdfs:label>
    <rdfs:domain rdf:resource="&pml-provenance;#MethodRule"/>
    <rdfs:range rdf:resource="&pml-provenance;#InferenceEngine"/>
  </owl:ObjectProperty>

  <owl:ObjectProperty rdf:about="#hasReport">
    <rdfs:comment xml:lang="en">Used to set the HTML report generated for a WDO or a SAW.</rdfs:comment>
    <rdfs:label xml:lang="en">has report</rdfs:label>
    <rdfs:domain rdf:resource="&owl;Ontology"/>
    <rdfs:range rdf:resource="&pml-provenance;#Website"/>
  </owl:ObjectProperty>

  <owl:ObjectProperty rdf:about="#hasSupportingDocumentation">
    <rdfs:comment xml:lang="en">Used to set supporting documentation for a SAW.</rdfs:comment>
    <rdfs:label xml:lang="en">has supporting documentation</rdfs:label>
    <rdfs:domain rdf:resource="#SemanticAbstractWorkflow"/>
    <rdfs:range rdf:resource="&pml-provenance;#Document"/>
  </owl:ObjectProperty>
</rdf:RDF>
